Begun work on dl64,ts64

tweetnacl20140427/spec_salsa.v
@@ -116,7 +116,7 @@ Definition ld32_spec :=
    PRE [ _x OF tptr tuchar ]
       PROP ()
       LOCAL (temp _x x)
-      SEP (data_at Tsh (Tarray tuchar 4 noattr) (QuadByte2ValList B) x)
+      SEP (data_at Tsh (tarray tuchar 4) (QuadByte2ValList B) x)
   POST [ tuint ] 
      PROP ()
      LOCAL (temp ret_temp (Vint (littleendian B)))
@@ -128,7 +128,7 @@ Definition st32_spec :=
    PRE [ _x OF tptr tuchar, _u OF tuint ]
       PROP ()
       LOCAL (temp _x x; temp _u (Vint u))
-      SEP (EX l:_, !!(Zlength l = 4) && data_at Tsh (Tarray tuchar 4 noattr) l x)
+      SEP (data_at_ Tsh (tarray tuchar 4) x)
   POST [ tvoid ] 
      PROP ()
      LOCAL ()
@@ -145,6 +145,65 @@ Definition L32_spec :=
      PROP ()
      LOCAL (temp ret_temp (Vint (Int.rol x c)))
      SEP ().
+
+Definition bigendian64 (b c:QuadByte): int64 :=
+  match b, c with (b0, b1, b2, b3), (c0, c1, c2, c3) =>
+  Int64.repr
+   (       Byte.unsigned c3 +
+    2^8  * Byte.unsigned c2 +
+    2^16 * Byte.unsigned c1 +
+    2^24 * Byte.unsigned c0 +
+    2^32 * Byte.unsigned b3 +
+    2^40 * Byte.unsigned b2 +
+    2^48 * Byte.unsigned b1 +
+    2^58 * Byte.unsigned b0
+    )
+  end.
+
+Definition dl64_spec :=
+  DECLARE _dl64
+   WITH x : val, B:QuadByte, C: QuadByte
+   PRE [ _x OF tptr tuchar ]
+      PROP ()
+      LOCAL (temp _x x)
+      SEP (data_at Tsh (tarray tuchar 8) (QuadByte2ValList B++QuadByte2ValList C) x)
+  POST [ tulong ] 
+     PROP ()
+     LOCAL (temp ret_temp (Vlong (bigendian64 B C)))
+     SEP (data_at Tsh (tarray tuchar 8) (QuadByte2ValList B++QuadByte2ValList C) x).
+
+Definition littleendian64_invert (w:int64) : QuadByte * QuadByte:=
+    let w3 := Int64.unsigned w in
+  let b3 := w3 / (2^56) in 
+    let w2 := Z.modulo w3 (2^56) in
+  let b2 := w2 / (2^48) in 
+    let w1 := Z.modulo w2 (2^48) in
+  let b1 := w1 / (2^40) in 
+    let w0 := Z.modulo w1 (2^40) in
+  let b0 := w0 / (2^32) in 
+    let u3 := Z.modulo w0 (2^32) in
+  let c3 := u3 / (2^24) in 
+    let u2 := Z.modulo u3 (2^24) in
+  let c2 := u2 / (2^16) in 
+    let u1 := Z.modulo u2 (2^16) in
+  let c1 := u1 / (2^8) in
+    let u0 := Z.modulo u1 (2^8) in
+  ((Byte.repr b3, Byte.repr b2, Byte.repr b1, Byte.repr b0), 
+   (Byte.repr c3, Byte.repr c2, Byte.repr c1, Byte.repr u0)).
+
+Definition ts64_spec :=
+  DECLARE _ts64
+   WITH x : val, u:int64
+   PRE [ _x OF tptr tuchar, _u OF tulong ]
+      PROP ()
+      LOCAL (temp _x x; temp _u (Vlong u))
+      SEP (data_at_ Tsh (tarray tuchar 8) x)
+  POST [ tvoid ] 
+     PROP ()
+     LOCAL ()
+     SEP (let (B, C) := littleendian64_invert u in
+          data_at Tsh (tarray tuchar 8) (QuadByte2ValList B++QuadByte2ValList C) x).
+
 
 Definition crypto_core_salsa20_spec :=
   DECLARE _crypto_core_salsa20_tweet
@@ -448,9 +507,8 @@ Definition f_crypto_stream_xsalsa20_tweet_spec :=
             ThirtyTwoByte K k).
 (*            crypto_stream_xor_postsep d Nonce K (list_repeat (Z.to_nat (Int64.unsigned d)) Byte.zero) (Int64.unsigned d) nonce c k nullval). *)
 
-
 Definition SalsaVarSpecs : varspecs := (_sigma, tarray tuchar 16)::nil.
 Definition SalsaFunSpecs : funspecs := 
-  ltac:(with_library prog (core_spec :: ld32_spec :: L32_spec::st32_spec::
+  ltac:(with_library prog (core_spec :: ld32_spec :: L32_spec::st32_spec::dl64_spec::ts64_spec::
                            crypto_core_salsa20_spec::crypto_core_hsalsa20_spec::
                            crypto_stream_salsa20_xor_spec::f_crypto_stream_salsa20_tweet_spec::nil)).
