tweetnacl20140427/verif_ld_st.v
@@ -86,23 +86,108 @@ Time entailer!.
   rewrite TP, BMU, Z.mul_add_distr_l, int_max_unsigned_eq. omega.
   rewrite TP, BMU, Z.mul_add_distr_l, int_max_unsigned_eq. omega.
 Time Qed. (*6.7*)
+(*
+Lemma dl64_spec_ok: semax_body SalsaVarSpecs SalsaFunSpecs
+       f_dl64 dl64_spec.
+Proof.
+start_function.
+destruct B as (((b0, b1), b2), b3).
+destruct C as (((c0, c1), c2), c3).
+unfold QuadByte2ValList; simpl. 
+specialize Byte_max_unsigned_Int_max_unsigned; intros BND.
+assert (RNGb3:= Byte.unsigned_range_2 b3).
+assert (RNGb2:= Byte.unsigned_range_2 b2).
+assert (RNGb1:= Byte.unsigned_range_2 b1).
+assert (RNGb0:= Byte.unsigned_range_2 b0).
+assert (RNGc3:= Byte.unsigned_range_2 c3).
+assert (RNGc2:= Byte.unsigned_range_2 c2).
+assert (RNGc1:= Byte.unsigned_range_2 c1).
+assert (RNGc0:= Byte.unsigned_range_2 c0).
+forward. simpl. rewrite Int.signed_repr.
+Parameter Data64: Z -> int64.
+forward_for_simple_bound 8 (EX i:Z, 
+  (PROP  ()
+   LOCAL (temp _x x; temp _u (Vlong (Data64 i)))
+   SEP (data_at Tsh (tarray tuchar 8)
+          (map Vint (map Int.repr (map Byte.unsigned 
+            [b0;b1;b2;b3;c0;c1;c2;c3]))) x))).
+{ entailer!. (*Data64 0 = 0*) admit. }
+{ rename H into I.
+  (*destruct (Znth_mapVint (map Int.repr
+                (map Byte.unsigned [b0; b1; b2; b3; c0; c1; c2; c3])) i Vundef)
+  as [d D]; simpl. apply I.*)
+  forward. 
+  + entailer!.
+    replace [Byte.unsigned b0; Byte.unsigned b1; Byte.unsigned b2;
+           Byte.unsigned b3; Byte.unsigned c0; Byte.unsigned c1;
+           Byte.unsigned c2; Byte.unsigned c3]
+    with (map Byte.unsigned [b0; b1; b2; b3; c0; c1; c2; c3]) by reflexivity.
+    rewrite Znth_map with (d':= Byte.zero).
+    rewrite zero_ext_inrange. rewrite Int.unsigned_repr. admit. admit. (*OK*)
+    rewrite Int.unsigned_repr. apply Byte.unsigned_range_2.
+    admit. (*OK*)
+    apply I.
+  + simpl. forward. entailer!. (*tc_error tulong int*) admit.
+    entailer!. admit. (*constraint on Data*) 
+}
+forward. apply prop_right. admit. (*condition on Data*)
+
+   Z0 _ i). _ Byte.unsigned). (Byte.unsigned [b0; b1; b2; b3; c0; c1; c2; c3].
+  rewrite Znth_map with (d':=Int.zero). simpl in D. rewrite D.  simpl. ucZnth_mapVint:
+data_at Tsh (tarray tuchar 4) 
+              (sublist 0 i (map Vint (map Int.repr (map Byte.unsigned ([u0;u1;u2;u3])))) ++ 
+               list_repeat (Z.to_nat(4-i)) Vundef)
+                x))).
+
+Time forward.
+time forward. (*1.8*)
+Time entailer!; omega. (*1.1*)
+Time forward. (*2*)
+Time entailer!; omega. (*1.1*)
+Time forward. (*1.1*)
+Time forward. (*2.2*)
+Time entailer!; omega. (*1.3*)
+Time forward. (*1.5*)
+drop_LOCAL 1%nat. 
+Time forward.
+Time entailer!; omega. (*1.3*)
+Time forward. (*5.2*)
+Time entailer!.
+  assert (WS: Int.zwordsize = 32). reflexivity.
+  assert (TP: two_p 8 = Byte.max_unsigned + 1). reflexivity.
+  assert (BMU: Byte.max_unsigned = 255). reflexivity. simpl.
+  repeat rewrite Int.shifted_or_is_add; try repeat rewrite Int.unsigned_repr; try omega.
+  f_equal. f_equal. simpl. 
+    rewrite Z.mul_add_distr_r. 
+    rewrite (Zmult_comm (Z.pow_pos 2 8)).
+    rewrite (Zmult_comm (Z.pow_pos 2 16)).
+    rewrite (Zmult_comm (Z.pow_pos 2 24)). 
+    simpl. repeat rewrite <- two_power_pos_correct.
+    rewrite Z.mul_add_distr_r.
+    rewrite Z.mul_add_distr_r.
+    repeat rewrite <- Z.mul_assoc. 
+    rewrite <- Z.add_assoc. rewrite <- Z.add_assoc. rewrite Z.add_comm. f_equal.
+    rewrite Z.add_comm. f_equal. rewrite Z.add_comm. f_equal.
+  rewrite TP, BMU, Z.mul_add_distr_l, int_max_unsigned_eq. omega. 
+  rewrite TP, BMU, Z.mul_add_distr_l, int_max_unsigned_eq. omega.
+  rewrite TP, BMU, Z.mul_add_distr_l, int_max_unsigned_eq. omega.
+Time Qed. (*6.7*)
+
 
 Lemma ST32_spec_ok: semax_body SalsaVarSpecs SalsaFunSpecs
        f_st32 st32_spec.
 Proof. 
-start_function.
-Intros l. rename H into Hl.
+start_function. 
 remember (littleendian_invert u) as U. destruct U as [[[u0 u1] u2] u3].
 
 Time forward_for_simple_bound 4 (EX i:Z, 
   (PROP  ()
    LOCAL (temp _x x; temp _u (Vint (iterShr8 u (Z.to_nat i))))
-   SEP (data_at Tsh (Tarray tuchar 4 noattr) 
+   SEP (data_at Tsh (tarray tuchar 4) 
               (sublist 0 i (map Vint (map Int.repr (map Byte.unsigned ([u0;u1;u2;u3])))) ++ 
-               sublist i (Zlength l) l)
+               list_repeat (Z.to_nat(4-i)) Vundef)
                 x))).
-(*0.9*)
-{ Time entailer!. (*1*) rewrite sublist_same; trivial. }
+{ entailer!. }
 { rename H into I.
   Time assert_PROP (field_compatible (Tarray tuchar 4 noattr) [] x /\ isptr x) 
        as FC_ptrX by solve [entailer!]. (*2.3*)
@@ -115,14 +200,9 @@ Time forward_for_simple_bound 4 (EX i:Z,
   autorewrite with sublist. 
   rewrite field_at_data_at. simpl. unfold field_address. simpl.
   if_tac. 2: solve [contradiction].
+  replace (4 - (1 + i)) with (4-i-1) by omega.
   rewrite isptr_offset_val_zero; trivial. clear H.
-  rewrite Zlength_length in Hl. 2: omega. 
-  destruct l; simpl in Hl. omega.
-        destruct l; simpl in Hl. omega.
-        destruct l; simpl in Hl. omega.
-        destruct l; simpl in Hl. omega.
-        destruct l; simpl in Hl. 2: solve [omega]. clear Hl.
-  apply data_at_ext.
+  apply data_at_ext. rewrite Zplus_comm.
         assert (ZW: Int.zwordsize = 32) by reflexivity.
         assert (EIGHT: Int.unsigned (Int.repr 8) = 8). apply Int.unsigned_repr. rewrite int_max_unsigned_eq; omega.
         inv HeqU. clear - ZW EIGHT I.
@@ -186,10 +266,343 @@ Time forward_for_simple_bound 4 (EX i:Z,
               rewrite zlt_true. repeat rewrite <- Z.add_assoc. reflexivity. omega. omega. omega. omega. omega.
           rewrite Int.bits_above. trivial. omega. }
         omega. }
-  rewrite Hl.
   Time forward. (*1.6*)
 Time Qed. (*4.9*) 
 
+Fixpoint iter64Shr8 (u : int64) (n : nat) {struct n} : int64 :=
+  match n with
+  | 0%nat => u
+  | S n' => Int64.shru (iter64Shr8 u n') (Int64.repr 8)
+  end.
+
+Lemma TS64_spec_ok: semax_body SalsaVarSpecs SalsaFunSpecs
+       f_ts64 ts64_spec.
+Proof. 
+start_function. 
+remember (littleendian64_invert u) as U. 
+destruct U as [W U]. destruct U as [[[u3 u2] u1] u0].
+destruct W as [[[w3 w2] w1] w0].
+(*unfold Sfor. forward. forward_seq.*)
+(*Parameter Data: Z -> list val.*)
+(*assert_PROP (isptr x) by entailer!. rename H into isptrX.*)
+Time forward_for_simple_bound 8 (EX i:Z, 
+  (PROP  ()
+   LOCAL (temp _x x; temp _u (Vlong (iter64Shr8 u (Z.to_nat i))))
+   SEP (data_at Tsh (tarray tuchar 8) 
+              (sublist 0 i (map Vint (map Int.repr (map Byte.unsigned ([u0;u1;u2;u3;w0;w1;w2;w3])))) ++ 
+               list_repeat (Z.to_nat(8-i)) Vundef)
+                x))).
+{ entailer!. }
+{ rename H into I.
+  Time assert_PROP (field_compatible (Tarray tuchar 8 noattr) [] x /\ isptr x) 
+       as FC_ptrX by solve [entailer!]. (*2.3*)
+  destruct FC_ptrX as [FC ptrX].
+  Time forward. apply andp_right. apply andp_right. solve [entailer!]. entailer. 
+        admit. (*!! typecheck_error (invalid_cast_result tuchar tuchar)*)
+        solve [entailer!]. 
+  Time forward. entailer. admit. (*another tc_error*)  
+  rewrite Z.add_comm, Z2Nat.inj_add; try omega.
+  Time entailer!. (*1.5*)
+  unfold upd_Znth.
+  autorewrite with sublist. 
+  rewrite field_at_data_at. simpl. unfold field_address. simpl.
+  if_tac. 2: solve [contradiction].
+  replace (8 - (1 + i)) with (8-i-1) by omega.
+  rewrite isptr_offset_val_zero; trivial. clear H.
+  apply data_at_ext. rewrite Zplus_comm.
+        assert (ZW: Int.zwordsize = 32) by reflexivity.
+        assert (EIGHT: Int.unsigned (Int.repr 8) = 8). apply Int.unsigned_repr. rewrite int_max_unsigned_eq; omega.
+        inv HeqU. clear - ZW EIGHT I. simpl.
+        destruct (zeq i 0); subst; simpl. f_equal. f_equal.
+        { rewrite Byte.unsigned_repr.              
+            rewrite (Fcore_Zaux.Zmod_mod_mult _ (2^8) (2^8)). 2: cbv; trivial. 2: cbv; intros; discriminate.
+            rewrite (Fcore_Zaux.Zmod_mod_mult _ (2^16) (2^8)). 2: cbv; trivial. 2: cbv; intros; discriminate.
+            rewrite <- (Int.zero_ext_mod 8).
+              rewrite Int.repr_unsigned; trivial.
+              rewrite ZW; omega.
+          assert (0 <= ((Int.unsigned u mod Z.pow_pos 2 24) mod Z.pow_pos 2 16) mod Z.pow_pos 2 8 < Byte.modulus).
+            apply Z_mod_lt. cbv; trivial. 
+            unfold Byte.max_unsigned. omega. }
+        destruct (zeq i 1); subst; simpl. f_equal. f_equal. f_equal.
+        { rewrite Byte.unsigned_repr.  
+          Focus 2. assert (0 <= (Int.unsigned u mod Z.pow_pos 2 24) mod Z.pow_pos 2 16 / Z.pow_pos 2 8 < Byte.modulus).
+                   Focus 2. unfold Byte.max_unsigned. omega.
+                   split. apply Z_div_pos. cbv; trivial. apply Z_mod_lt. cbv; trivial.
+                   apply Zdiv_lt_upper_bound. cbv; trivial. apply Z_mod_lt. cbv; trivial.
+          apply Int.same_bits_eq. rewrite ZW; intros.
+          rewrite Int.bits_zero_ext, Int.testbit_repr; try apply H. 
+          rewrite (Z.div_pow2_bits _ 8); try omega.
+          rewrite (Int.Ztestbit_mod_two_p 16); try omega.
+          rewrite (Int.Ztestbit_mod_two_p 24); try omega.
+          rewrite Int.bits_shru; try omega. rewrite EIGHT, ZW, Ztest_Inttest.
+          remember (zlt i 8). 
+          destruct s. repeat rewrite zlt_true. trivial. omega. omega. omega.
+          rewrite zlt_false. trivial. omega. }
+        destruct (zeq i 2); subst; simpl. f_equal. f_equal. f_equal.
+          f_equal.
+        { rewrite Byte.unsigned_repr.  
+          Focus 2. assert (0 <= Int.unsigned u mod Z.pow_pos 2 24 / Z.pow_pos 2 16 < Byte.modulus).
+                   2: unfold Byte.max_unsigned; omega.
+                   split. apply Z_div_pos. cbv; trivial. apply Z_mod_lt. cbv; trivial.
+                   apply Zdiv_lt_upper_bound. cbv; trivial. apply Z_mod_lt. cbv; trivial.
+          apply Int.same_bits_eq. rewrite ZW; intros.
+          rewrite Int.bits_zero_ext, Int.testbit_repr; try apply H. 
+          rewrite Int.bits_shru; try omega. rewrite EIGHT, ZW.
+          rewrite (Z.div_pow2_bits _ 16); try omega.
+          rewrite (Int.Ztestbit_mod_two_p 24); try omega.
+          rewrite Ztest_Inttest.
+          remember (zlt i 8). 
+          destruct s. repeat rewrite zlt_true. rewrite Int.bits_shru, EIGHT, ZW.
+              rewrite zlt_true. rewrite <- Z.add_assoc. reflexivity. omega. omega. omega. omega.
+          rewrite zlt_false. trivial. omega. }
+        destruct (zeq i 3); subst; simpl. f_equal. f_equal. f_equal. f_equal.
+          f_equal.
+        { rewrite Byte.unsigned_repr.  
+          Focus 2. assert (0 <= Int.unsigned u / Z.pow_pos 2 24 < Byte.modulus).
+                   2: unfold Byte.max_unsigned; omega.
+                   split. apply Z_div_pos. cbv; trivial. apply Int.unsigned_range. 
+                   apply Zdiv_lt_upper_bound. cbv; trivial. apply Int.unsigned_range. 
+          apply Int.same_bits_eq. rewrite ZW; intros.
+          rewrite Int.bits_zero_ext, Int.testbit_repr; try apply H. 
+          rewrite Int.bits_shru; try omega. rewrite EIGHT, ZW.
+          rewrite (Z.div_pow2_bits _ 24); try omega.
+          rewrite Ztest_Inttest.
+          remember (zlt i 8). 
+          destruct s. rewrite zlt_true. rewrite Int.bits_shru, EIGHT, ZW.
+              rewrite zlt_true. rewrite Int.bits_shru, EIGHT, ZW. 
+              rewrite zlt_true. repeat rewrite <- Z.add_assoc. reflexivity. omega. omega. omega. omega. omega.
+          rewrite Int.bits_above. trivial. omega. }
+        omega. }
+  Time forward. (*1.6*)
+Time Qed. (*4.9*) 
+
+ unfold data_at_, field_at_.
+  rewrite field_at_data_at. 
+  rewrite field_address_offset by auto with field_compatible. simpl.
+  rewrite isptr_offset_val_zero. apply data_at_ext. unfold default_val. simpl. unfold tarray. simpl.   destruct tv. reflexivity. cancel. rewrite unfold field_address; simpl. normalize. cancel. }
+
+forward_for (EX z:_, 
+  (PROP (0<= z <= 7 )
+   LOCAL (temp _i (Vint (Int.repr z)); temp _x x; 
+          temp _u (Vlong u))
+   SEP (data_at Tsh (tarray tuchar 8) (Data z) x))). 
+{ Exists 7. entailer!. admit. (*Data 7 = list_repeat 8 Vundef*) }
+
+eapply semax_for with (A:=Z)(v:= fun a => Val.of_bool (negb (Int.lt (Int.repr a) (Int.repr 0)))).
+ solve [ reflexivity].
+ intros. solve [entailer!].
+ intros. entailer!. 
+{ intros i. simpl. normalize. rename H into I0. rename H0 into I7.
+  apply negb_true_iff in I0. (* apply lt_repr_false in I0. 
+   2: red; unfold Int.min_signed, Int.max_signed; simpl. 2: split; try omega. Focus 2.
+   2: red; unfold Int.min_signed, Int.max_signed; simpl; omega.*)
+
+ forward.
+  { apply andp_right. 2: solve [entailer].
+    apply andp_right. solve [entailer!].
+    entailer. admit. (*typecheck_error (invalid_cast_result tuchar tuchar)*) }
+
+  forward. entailer. simpl. admit. (*typecheck_error
+         (arg_type
+            (Ebinop Oshr (Etempvar _u tulong) (Econst_int (Int.repr 8) tint)
+               tulong))*)
+
+  
+  unfold arg_type.
+ go_lower. entailer!. Search invalid_cast_result. unfold invalid_cast_result. typecheck_error. simpl.  simpl. destruct (zlt   
+{ apply extract_exists_pre. intros i. Intros. rename H into I.
+  
+ cancel. Focus 2. eapply semax_for with (A:=Z).
+  reflexivity.
+Ltac forward_for_simple_bound n Pre ::=
+  check_Delta;
+ repeat match goal with |-
+      semax _ _ (Ssequence (Ssequence (Ssequence _ _) _) _) _ =>
+      apply -> seq_assoc; abbreviate_semax
+ end. (*
+ first [ 
+    match type of n with
+      ?t => first [ unify t Z | elimtype (Type_of_bound_in_forward_for_should_be_Z_but_is t)]
+    end;
+    match type of Pre with
+      ?t => first [unify t (environ -> mpred); fail 1 | elimtype (Type_of_invariant_in_forward_for_should_be_environ_arrow_mpred_but_is t)]
+    end
+  | simple eapply semax_seq'; 
+    [forward_for_simple_bound' n Pre 
+    | cbv beta; simpl update_tycon; abbreviate_semax  ]
+  | eapply semax_post_flipped'; 
+     [forward_for_simple_bound' n Pre 
+     | ]
+  ].*)
+
+Time forward_for_simple_bound 8 (EX i:Z, 
+  (PROP  ()
+   LOCAL (temp _x x; temp _u (Vlong (iter64Shr8 u (Z.to_nat i))))
+   SEP (data_at Tsh (tarray tuchar 8) 
+              (sublist 0 i (map Vint (map Int.repr (map Byte.unsigned ([w0;w1;w2;w3;u0;u1;u2;u3])))) ++ 
+               list_repeat (Z.to_nat(8-i)) Vundef)
+                x))).
+{ entailer!. }
+{ rename H into I.
+  Time assert_PROP (field_compatible (Tarray tuchar 4 noattr) [] x /\ isptr x) 
+       as FC_ptrX by solve [entailer!]. (*2.3*)
+  destruct FC_ptrX as [FC ptrX].
+  Time forward. (*3.2*)
+  Time forward. (*0.8*)  
+  rewrite Z.add_comm, Z2Nat.inj_add; try omega.
+  Time entailer!. (*1.5*)
+  unfold upd_Znth.
+  autorewrite with sublist. 
+  rewrite field_at_data_at. simpl. unfold field_address. simpl.
+  if_tac. 2: solve [contradiction].
+  replace (4 - (1 + i)) with (4-i-1) by omega.
+  rewrite isptr_offset_val_zero; trivial. clear H.
+  apply data_at_ext. rewrite Zplus_comm.
+        assert (ZW: Int.zwordsize = 32) by reflexivity.
+        assert (EIGHT: Int.unsigned (Int.repr 8) = 8). apply Int.unsigned_repr. rewrite int_max_unsigned_eq; omega.
+        inv HeqU. clear - ZW EIGHT I.
+        destruct (zeq i 0); subst; simpl. f_equal. f_equal.
+        { rewrite Byte.unsigned_repr.              
+            rewrite (Fcore_Zaux.Zmod_mod_mult _ (2^8) (2^8)). 2: cbv; trivial. 2: cbv; intros; discriminate.
+            rewrite (Fcore_Zaux.Zmod_mod_mult _ (2^16) (2^8)). 2: cbv; trivial. 2: cbv; intros; discriminate.
+            rewrite <- (Int.zero_ext_mod 8).
+              rewrite Int.repr_unsigned; trivial.
+              rewrite ZW; omega.
+          assert (0 <= ((Int.unsigned u mod Z.pow_pos 2 24) mod Z.pow_pos 2 16) mod Z.pow_pos 2 8 < Byte.modulus).
+            apply Z_mod_lt. cbv; trivial. 
+            unfold Byte.max_unsigned. omega. }
+        destruct (zeq i 1); subst; simpl. f_equal. f_equal. f_equal.
+        { rewrite Byte.unsigned_repr.  
+          Focus 2. assert (0 <= (Int.unsigned u mod Z.pow_pos 2 24) mod Z.pow_pos 2 16 / Z.pow_pos 2 8 < Byte.modulus).
+                   Focus 2. unfold Byte.max_unsigned. omega.
+                   split. apply Z_div_pos. cbv; trivial. apply Z_mod_lt. cbv; trivial.
+                   apply Zdiv_lt_upper_bound. cbv; trivial. apply Z_mod_lt. cbv; trivial.
+          apply Int.same_bits_eq. rewrite ZW; intros.
+          rewrite Int.bits_zero_ext, Int.testbit_repr; try apply H. 
+          rewrite (Z.div_pow2_bits _ 8); try omega.
+          rewrite (Int.Ztestbit_mod_two_p 16); try omega.
+          rewrite (Int.Ztestbit_mod_two_p 24); try omega.
+          rewrite Int.bits_shru; try omega. rewrite EIGHT, ZW, Ztest_Inttest.
+          remember (zlt i 8). 
+          destruct s. repeat rewrite zlt_true. trivial. omega. omega. omega.
+          rewrite zlt_false. trivial. omega. }
+        destruct (zeq i 2); subst; simpl. f_equal. f_equal. f_equal.
+          f_equal.
+        { rewrite Byte.unsigned_repr.  
+          Focus 2. assert (0 <= Int.unsigned u mod Z.pow_pos 2 24 / Z.pow_pos 2 16 < Byte.modulus).
+                   2: unfold Byte.max_unsigned; omega.
+                   split. apply Z_div_pos. cbv; trivial. apply Z_mod_lt. cbv; trivial.
+                   apply Zdiv_lt_upper_bound. cbv; trivial. apply Z_mod_lt. cbv; trivial.
+          apply Int.same_bits_eq. rewrite ZW; intros.
+          rewrite Int.bits_zero_ext, Int.testbit_repr; try apply H. 
+          rewrite Int.bits_shru; try omega. rewrite EIGHT, ZW.
+          rewrite (Z.div_pow2_bits _ 16); try omega.
+          rewrite (Int.Ztestbit_mod_two_p 24); try omega.
+          rewrite Ztest_Inttest.
+          remember (zlt i 8). 
+          destruct s. repeat rewrite zlt_true. rewrite Int.bits_shru, EIGHT, ZW.
+              rewrite zlt_true. rewrite <- Z.add_assoc. reflexivity. omega. omega. omega. omega.
+          rewrite zlt_false. trivial. omega. }
+        destruct (zeq i 3); subst; simpl. f_equal. f_equal. f_equal. f_equal.
+          f_equal.
+        { rewrite Byte.unsigned_repr.  
+          Focus 2. assert (0 <= Int.unsigned u / Z.pow_pos 2 24 < Byte.modulus).
+                   2: unfold Byte.max_unsigned; omega.
+                   split. apply Z_div_pos. cbv; trivial. apply Int.unsigned_range. 
+                   apply Zdiv_lt_upper_bound. cbv; trivial. apply Int.unsigned_range. 
+          apply Int.same_bits_eq. rewrite ZW; intros.
+          rewrite Int.bits_zero_ext, Int.testbit_repr; try apply H. 
+          rewrite Int.bits_shru; try omega. rewrite EIGHT, ZW.
+          rewrite (Z.div_pow2_bits _ 24); try omega.
+          rewrite Ztest_Inttest.
+          remember (zlt i 8). 
+          destruct s. rewrite zlt_true. rewrite Int.bits_shru, EIGHT, ZW.
+              rewrite zlt_true. rewrite Int.bits_shru, EIGHT, ZW. 
+              rewrite zlt_true. repeat rewrite <- Z.add_assoc. reflexivity. omega. omega. omega. omega. omega.
+          rewrite Int.bits_above. trivial. omega. }
+        omega. }
+  Time forward. (*1.6*)
+Time Qed. (*4.9*) 
+
+Lemma dl64_spec_ok: semax_body SalsaVarSpecs SalsaFunSpecs
+       f_dl64 dl64_spec.
+Proof.
+start_function.
+destruct B as (((b3, b2), b1), b0). 
+destruct C as (((c3, c2), c1), c0). simpl.
+assert (BND: Byte.max_unsigned < Int64.max_unsigned) by (cbv; trivial). 
+assert (RNGB3:= Byte.unsigned_range_2 b3).
+assert (RNGB2:= Byte.unsigned_range_2 b2).
+assert (RNGB1:= Byte.unsigned_range_2 b1).
+assert (RNGB0:= Byte.unsigned_range_2 b0). 
+assert (RNGC3:= Byte.unsigned_range_2 c3).
+assert (RNGC2:= Byte.unsigned_range_2 c2).
+assert (RNGC1:= Byte.unsigned_range_2 c1).
+assert (RNGC0:= Byte.unsigned_range_2 c0).
+forward. simpl. 
+Parameter myval:Z -> Z.
+unfold Sfor.
+forward.
+forward_seq.
+eapply semax_pre.
+Focus 2.
+eapply semax_for with (A:=Z)(v:=fun a=>Vint (Int.repr a)).
+  solve [ reflexivity ].
+  solve [ intros; entailer ]. simpl.
+  solve [ intros; entailer ].
+Time forward_for_simple_bound 8 (EX i:Z, 
+  (PROP ( )
+   LOCAL (temp _u (Vlong (Int64.repr (myval i))); 
+          temp _x x)
+   SEP (data_at Tsh (tarray tuchar 8)
+          (Vint (Int.repr (Byte.unsigned b3))
+           :: Vint (Int.repr (Byte.unsigned b2))
+              :: Vint (Int.repr (Byte.unsigned b1))
+                 :: Vint (Int.repr (Byte.unsigned b0))
+                    :: QuadByte2ValList (c3, c2, c1, c0)) x))).
+
+  (PROP  ()
+   LOCAL (temp _x x; temp _u (Vint (iterShr8 u (Z.to_nat i))))
+   SEP (data_at Tsh (tarray tuchar 4) 
+              (sublist 0 i (map Vint (map Int.repr (map Byte.unsigned ([u0;u1;u2;u3])))) ++ 
+               list_repeat (Z.to_nat(4-i)) Vundef)
+                x))).
+{ entailer!. }
+
+Time forward.
+Time forward. (*1.8*)
+Time entailer!; omega. (*1.1*)
+Time forward. (*2*)
+Time entailer!; omega. (*1.1*)
+Time forward. (*1.1*)
+Time forward. (*2.2*)
+Time entailer!; omega. (*1.3*)
+Time forward. (*1.5*)
+drop_LOCAL 1%nat. 
+Time forward.
+Time entailer!; omega. (*1.3*)
+Time forward. (*5.2*)
+Time entailer!.
+  assert (WS: Int.zwordsize = 32). reflexivity.
+  assert (TP: two_p 8 = Byte.max_unsigned + 1). reflexivity.
+  assert (BMU: Byte.max_unsigned = 255). reflexivity. simpl.
+  repeat rewrite Int.shifted_or_is_add; try repeat rewrite Int.unsigned_repr; try omega.
+  f_equal. f_equal. simpl. 
+    rewrite Z.mul_add_distr_r. 
+    rewrite (Zmult_comm (Z.pow_pos 2 8)).
+    rewrite (Zmult_comm (Z.pow_pos 2 16)).
+    rewrite (Zmult_comm (Z.pow_pos 2 24)). 
+    simpl. repeat rewrite <- two_power_pos_correct.
+    rewrite Z.mul_add_distr_r.
+    rewrite Z.mul_add_distr_r.
+    repeat rewrite <- Z.mul_assoc. 
+    rewrite <- Z.add_assoc. rewrite <- Z.add_assoc. rewrite Z.add_comm. f_equal.
+    rewrite Z.add_comm. f_equal. rewrite Z.add_comm. f_equal.
+  rewrite TP, BMU, Z.mul_add_distr_l, int_max_unsigned_eq. omega. 
+  rewrite TP, BMU, Z.mul_add_distr_l, int_max_unsigned_eq. omega.
+  rewrite TP, BMU, Z.mul_add_distr_l, int_max_unsigned_eq. omega.
+Time Qed. (*6.7*)
+*)
 (*
 Definition L32_specZ :=
   DECLARE _L32
